Respect some oracle for resource inv domains
When releasing, the memory returned will follow a policy, and we
parametrize our semantics over that policy. This makes it possible to
prove that the resource invariant is preserved, since you have some
control over what memory is returned.

src/CSL.v
@@ -21,8 +21,18 @@ Section ConcurrentSepLogic.
   (** We will define programs that return T. *)
   Variable T:Type.
 
-  Implicit Types r : R.
+  (** The execution semantics will release memory for resources according to this
+      policy. in_resource_domain r m a should hold when the resource invariant of r
+      should include a in memory m. *)
+  Variable in_resource_domain : R -> @mem addr (@weq addrlen) valu ->
+                                (addr -> Prop).
+
+
+  Implicit Type r : R.
   Implicit Types m rm : @mem addr (@weq addrlen) valu.
+
+  Definition respects_domain r m rm :=
+    (forall a, in_resource_domain r m a -> exists v, rm a = Some v).
 
   (* TODO: change state to capture p and locks, not m and locks *)
   Inductive state :=
@@ -62,6 +72,7 @@ Section ConcurrentSepLogic.
   | SRel : forall m m' rm ls r rx,
       mem_disjoint m' rm ->
       m = mem_union m' rm ->
+      respects_domain r m rm ->
       rstep (State m ls) (Rel r rx)
             (State m (remove REQ r ls)) (rx tt)
             [RelStep r rm].
@@ -83,43 +94,97 @@ Section ConcurrentSepLogic.
 
   Hint Constructors rexec.
 
-  Theorem rexec_progress : forall p s,
-      exists events out,
-        rexec s p events out.
+  Ltac inv_state :=
+    match goal with
+    | [ H: @eq state ?a ?b |- _ ] =>
+      inversion H; subst; clear H
+    end.
+
+  Ltac inv_rstep :=
+    match goal with
+    | [ H : rstep _ _ _ _ _ |- _ ] =>
+      inversion H; subst
+    end.
+
+  Lemma read_failure : forall m a ls rx,
+      m a = None ->
+      rexec (State m ls) (CRead a rx) nil Failed.
   Proof.
-    induction p; destruct s; eauto.
-    - case_eq (m a); intros.
-      * evar (s: state).
-        specialize (H w ?s).
-        repeat deex; repeat eexists.
-        eauto.
-      * repeat eexists; eapply EFail; intros.
-        intro.
-        inversion H1; congruence.
-        congruence.
-    - case_eq (m a); intros.
-      * evar (s: state).
-        specialize (H tt ?s).
-        repeat deex; repeat eexists.
-        eauto.
-      * repeat eexists; eapply EFail; intros.
-        intro.
-        inversion H1; congruence.
-        congruence.
-    - Hint Resolve mem_disjoint_empty_mem_r.
-      evar (s: state).
-      specialize (H tt ?s).
+    intros.
+    eapply EFail; try congruence; intros.
+    intro.
+    inv_rstep; congruence.
+  Qed.
+
+  Lemma write_failure : forall m a v ls rx,
+      m a = None ->
+      rexec (State m ls) (CWrite a v rx) nil Failed.
+  Proof.
+    intros.
+    eapply EFail; try congruence; intros.
+    intro.
+    inv_rstep; congruence.
+  Qed.
+
+  (** Instantiate a forall hypothesis with fresh evars.
+      If H quantifies over a Prop and a proof is in context,
+      we instantiate to that proof (following proof irrelevance). *)
+  Ltac specialize_evars H :=
+    repeat match type of H with
+    | (forall x:?T, _) =>
+      match type of T with
+      (* H looks like forall H', ...; if we can find an H', then use that
+         directly *)
+      | Prop =>
+        match goal with
+        | [ H' : T |- _ ] =>
+          specialize (H H')
+        end
+      (* normal case: create an evar and specialize to it *)
+      | _ =>
+        let x := fresh x in
+        evar (x:T);
+          specialize (H x);
+          (* a quirk of evar is that it creates a variable and an evar;
+             from Ltac it doesn't seem like we can access the evar name,
+             but we can simply get rid of the variable with subst. *)
+          subst x
+      end
+    end.
+
+  Theorem rexec_progress : forall p m locks,
+      (* this is a very powerful hypothesis, but in general if in_resource_domain looks
+         at the memory contents, then Writes could get us into a state where
+         there's no way to release memory that even has the right domain.
+
+         In these cases, if in_resource_domain is at least decidable, then we can still
+         prove progress via a fail step. *)
+      (forall r m, exists m' rm, m = mem_union m' rm /\
+                       mem_disjoint m' rm /\
+                       respects_domain r m rm) ->
+      exists events out,
+        rexec (State m locks) p events out.
+  Proof.
+    Local Hint Resolve read_failure write_failure.
+    induction p; intros; eauto.
+    - case_eq (m a); intros; eauto.
+      specialize_evars H.
+      repeat deex; repeat eexists.
+      eauto.
+    - case_eq (m a); intros; eauto.
+      specialize_evars H.
+      repeat deex; repeat eexists.
+      eauto.
+    - specialize_evars H.
+      repeat deex.
+      repeat eexists; eauto.
+      econstructor; eauto.
+      econstructor.
+      apply mem_disjoint_empty_mem_r.
+    - specialize_evars H.
+      specialize_evars H0.
       repeat deex.
       do 2 eexists; eauto.
-    - evar (s: state).
-      specialize (H tt ?s).
-      repeat deex.
-      do 2 eexists; eauto.
-      econstructor.
-      econstructor.
-      eauto.
-      rewrite mem_union_empty_mem_r; reflexivity.
-      eauto.
   Qed.
 
   Definition donecond :=  T -> @pred addr (@weq addrlen) valu.
@@ -182,21 +247,9 @@ Section ConcurrentSepLogic.
     e1 binder, e2 binder,
     only parsing).
 
-  Ltac inv_rstep :=
-    match goal with
-    | [ H : rstep _ _ _ _ _ |- _ ] =>
-      inversion H; subst
-    end.
-
   Ltac inv_cprog :=
     match goal with
     | [ H: @eq cprog ?a ?b |- _ ] =>
-      inversion H; subst; clear H
-    end.
-
-  Ltac inv_state :=
-    match goal with
-    | [ H: @eq state ?a ?b |- _ ] =>
       inversion H; subst; clear H
     end.
 
@@ -374,6 +427,5 @@ Section ConcurrentSepLogic.
             P} (CWrite a va) , (CWrite b vb).
   Proof.
   Admitted.
-
 
 End ConcurrentSepLogic.
